ConNF.lean
@@ -5,6 +5,7 @@ import ConNF.Aux.Set
 import ConNF.Aux.Transfer
 import ConNF.Aux.WellOrder
 import ConNF.FOA.Approximates
+import ConNF.FOA.BaseAction
 import ConNF.FOA.BaseApprox
 import ConNF.FOA.StrApprox
 import ConNF.Setup.Atom
