ConNF/FOA/BaseAction.lean
@@ -1,0 +1,161 @@
+import ConNF.Setup.NearLitter
+
+/-!
+# Base actions
+
+In this file, we define base actions.
+
+## Main declarations
+
+* `ConNF.BaseAction`: The type of base actions.
+-/
+
+noncomputable section
+universe u
+
+open Cardinal Ordinal
+open scoped symmDiff
+
+namespace ConNF
+
+variable [Params.{u}]
+
+structure BaseAction where
+  atoms : Rel Atom Atom
+  nearLitters : Rel NearLitter NearLitter
+  atoms_dom_small' : Small atoms.dom
+  nearLitters_dom_small' : Small nearLitters.dom
+  atoms_oneOne' : atoms.OneOne
+  mem_iff_mem' {a₁ a₂ : Atom} {N₁ N₂ : NearLitter} :
+    atoms a₁ a₂ → nearLitters N₁ N₂ → (a₁ ∈ N₁ᴬ ↔ a₂ ∈ N₂ᴬ)
+  litter_eq_litter_iff' {N₁ N₂ N₃ N₄ : NearLitter} :
+    nearLitters N₁ N₃ → nearLitters N₂ N₄ → (N₁ᴸ = N₂ᴸ ↔ N₃ᴸ = N₄ᴸ)
+  interference_subset_dom' {N₁ N₂ : NearLitter} :
+    N₁ ∈ nearLitters.dom → N₂ ∈ nearLitters.dom → interference N₁ N₂ ⊆ atoms.dom
+  interference_subset_codom' {N₁ N₂ : NearLitter} :
+    N₁ ∈ nearLitters.codom → N₂ ∈ nearLitters.codom → interference N₁ N₂ ⊆ atoms.codom
+
+namespace BaseAction
+
+instance : SuperA BaseAction (Rel Atom Atom) where
+  superA := atoms
+
+instance : SuperN BaseAction (Rel NearLitter NearLitter) where
+  superN := nearLitters
+
+theorem atoms_dom_small (ξ : BaseAction) : Small ξᴬ.dom :=
+  ξ.atoms_dom_small'
+
+theorem nearLitters_dom_small (ξ : BaseAction) : Small ξᴺ.dom :=
+  ξ.nearLitters_dom_small'
+
+theorem atoms_oneOne (ξ : BaseAction) : ξᴬ.OneOne :=
+  ξ.atoms_oneOne'
+
+theorem mem_iff_mem {ξ : BaseAction} {a₁ a₂ : Atom} {N₁ N₂ : NearLitter} :
+    ξᴬ a₁ a₂ → ξᴺ N₁ N₂ → (a₁ ∈ N₁ᴬ ↔ a₂ ∈ N₂ᴬ) :=
+  ξ.mem_iff_mem'
+
+theorem litter_eq_litter_iff {ξ : BaseAction} {N₁ N₂ N₃ N₄ : NearLitter} :
+    ξᴺ N₁ N₃ → ξᴺ N₂ N₄ → (N₁ᴸ = N₂ᴸ ↔ N₃ᴸ = N₄ᴸ) :=
+  ξ.litter_eq_litter_iff'
+
+theorem interference_subset_dom {ξ : BaseAction} {N₁ N₂ : NearLitter} :
+    N₁ ∈ ξᴺ.dom → N₂ ∈ ξᴺ.dom → interference N₁ N₂ ⊆ ξᴬ.dom :=
+  ξ.interference_subset_dom'
+
+theorem interference_subset_codom {ξ : BaseAction} {N₁ N₂ : NearLitter} :
+    N₁ ∈ ξᴺ.codom → N₂ ∈ ξᴺ.codom → interference N₁ N₂ ⊆ ξᴬ.codom :=
+  ξ.interference_subset_codom'
+
+theorem mem_symmDiff_iff_mem_symmDiff {ξ : BaseAction} {a₁ a₂ : Atom} {N₁ N₂ N₃ N₄ : NearLitter} :
+    ξᴬ a₁ a₂ → ξᴺ N₁ N₂ → ξᴺ N₃ N₄ → (a₁ ∈ N₁ᴬ ∆ N₃ᴬ ↔ a₂ ∈ N₂ᴬ ∆ N₄ᴬ) := by
+  intro ha hN₁₂ hN₃₄
+  simp only [Set.mem_symmDiff, mem_iff_mem ha hN₁₂, mem_iff_mem ha hN₃₄]
+
+theorem nearLitters_coinjective (ξ : BaseAction) : ξᴺ.Coinjective := by
+  constructor
+  intro N₁ N₂ N h₁ h₂
+  apply NearLitter.ext
+  rw [← Set.symmDiff_eq_empty, Set.eq_empty_iff_forall_not_mem]
+  intro a ha
+  have := interference_subset_codom ⟨_, h₁⟩ ⟨_, h₂⟩
+  rw [interference_eq_of_litter_eq ((litter_eq_litter_iff h₁ h₂).mp rfl)] at this
+  obtain ⟨b, hba⟩ := this ha
+  rw [← mem_symmDiff_iff_mem_symmDiff hba h₁ h₂] at ha
+  simp only [symmDiff_self, Set.bot_eq_empty, Set.mem_empty_iff_false] at ha
+
+theorem atoms_codom_small (ξ : BaseAction) : Small ξᴬ.codom :=
+  small_codom_of_small_dom ξ.atoms_oneOne.toCoinjective ξ.atoms_dom_small
+
+theorem nearLitters_codom_small (ξ : BaseAction) : Small ξᴺ.codom :=
+  small_codom_of_small_dom ξ.nearLitters_coinjective ξ.nearLitters_dom_small
+
+def inv (ξ : BaseAction) : BaseAction where
+  atoms := ξᴬ.inv
+  nearLitters := ξᴺ.inv
+  atoms_dom_small' := ξ.atoms_codom_small
+  nearLitters_dom_small' := ξ.nearLitters_codom_small
+  atoms_oneOne' := ξ.atoms_oneOne.inv
+  mem_iff_mem' h₁ h₂ := (ξ.mem_iff_mem h₁ h₂).symm
+  litter_eq_litter_iff' h₁ h₂ := (ξ.litter_eq_litter_iff h₁ h₂).symm
+  interference_subset_dom' := ξ.interference_subset_codom
+  interference_subset_codom' := ξ.interference_subset_dom
+
+instance : Inv BaseAction where
+  inv := inv
+
+@[simp]
+theorem inv_atoms (ξ : BaseAction) : ξ⁻¹ᴬ = ξᴬ.inv :=
+  rfl
+
+@[simp]
+theorem inv_nearLitters (ξ : BaseAction) : ξ⁻¹ᴺ = ξᴺ.inv :=
+  rfl
+
+theorem nearLitters_injective (ξ : BaseAction) : ξᴺ.Injective := by
+  have := ξ⁻¹.nearLitters_coinjective
+  rwa [inv_nearLitters, Rel.inv_coinjective_iff] at this
+
+theorem nearLitters_oneOne (ξ : BaseAction) : ξᴺ.OneOne :=
+  ⟨ξ.nearLitters_injective, ξ.nearLitters_coinjective⟩
+
+inductive litters (ξ : BaseAction) : Rel Litter Litter
+  | mk {N₁ N₂ : NearLitter} : ξᴺ N₁ N₂ → ξ.litters N₁ᴸ N₂ᴸ
+
+instance : SuperL BaseAction (Rel Litter Litter) where
+  superL := litters
+
+theorem litters_iff {ξ : BaseAction} (L₁ L₂ : Litter) :
+    ξᴸ L₁ L₂ ↔ ∃ N₁ N₂, N₁ᴸ = L₁ ∧ N₂ᴸ = L₂ ∧ ξᴺ N₁ N₂ := by
+  constructor
+  · rintro ⟨⟩
+    refine ⟨_, _, rfl, rfl, ?_⟩
+    assumption
+  · rintro ⟨N₁, N₂, rfl, rfl, h⟩
+    exact ⟨h⟩
+
+theorem litters_coinjective (ξ : BaseAction) : ξᴸ.Coinjective := by
+  constructor
+  intro L₁ L₂ L h₁ h₂
+  rw [litters_iff] at h₁ h₂
+  obtain ⟨N₃, N₁, h₃, rfl, h₁⟩ := h₁
+  obtain ⟨N₄, N₂, h₄, rfl, h₂⟩ := h₂
+  exact (litter_eq_litter_iff h₁ h₂).mp (h₃.trans h₄.symm)
+
+@[simp]
+theorem inv_litters (ξ : BaseAction) : ξ⁻¹ᴸ = ξᴸ.inv := by
+  ext L₁ L₂
+  simp only [litters_iff, inv_nearLitters, exists_and_left, Rel.inv_def]
+  tauto
+
+theorem litters_injective (ξ : BaseAction) : ξᴸ.Injective := by
+  have := ξ⁻¹.litters_coinjective
+  rwa [inv_litters, Rel.inv_coinjective_iff] at this
+
+theorem litters_oneOne (ξ : BaseAction) : ξᴸ.OneOne :=
+  ⟨ξ.litters_injective, ξ.litters_coinjective⟩
+
+end BaseAction
+
+end ConNF
